translation/Translation.v
@@ -1,0 +1,18 @@
+Require Import Predefs.
+Require Import TLC.LibTactics.
+
+(* lemma from https://stackoverflow.com/q/27322979/1296238 *)
+Lemma ex_falso: forall T: Type, False -> T.
+  inversion 1.
+Qed.
+
+Definition translator : translation_type.
+  unfold translation_type.
+  intro.
+  induction t; introv; intros okGadt Htyp.
+  - apply ex_falso. inversion Htyp.
+  - apply ex_falso. inversion Htyp; subst.
+    admit.
+  - admit.
+  - econstructor.
+Admitted.
